examples/uint63nat/prims_verif.v
@@ -30,10 +30,19 @@ Qed.
 Lemma body_uint63_add:
   semax_body Vprog Gprog f_uint63_add uint63_add_spec.
 Proof. 
-  start_function. 
-  forward. entailer!.
+start_function1.
+repeat (simple apply intro_prop_through_close_precondition; intro).
+concretize_PARAMS.
+(* TODO: FIX *)
+destruct xs. unfold prim_in_graphs in H1. simpl in H1. destruct ps; try contradiction.
+destruct H1. subst.
+start_function2. 
+start_function3.
+forward.
+ entailer!.
   unfold encode_Z in *.
-  autorewrite with norm. rewrite !Int64.shru_div_two_p.
+  autorewrite with norm.
+(*   rewrite !Int64.shru_div_two_p.
 change (two_p _) with 2.
 rewrite !Int64.unsigned_repr by lia.  
 rewrite Z.div_add_l by lia.
@@ -45,12 +54,14 @@ assert ((Z.of_nat n * 2 + 1) / 2 = Z.of_nat n) as ->.
   replace (1/2) with 0 by reflexivity. 
   lia. }
 lia. 
-Qed.
+Qed. *)
+Admitted.
 
 Lemma body_uint63_from_nat:
   semax_body Vprog Gprog f_uint63_from_nat uint63_from_nat_spec.
 Proof.
- start_function. 
+ start_function'. 
+ rename x into n.
  forward.
  fold (rep_type_val g p).
  forward.
@@ -62,10 +73,10 @@ Proof.
         LOCAL (temp _i (Vlong (Int64.repr (Z.of_nat m))); 
                temp _temp (rep_type_val g p');
                temp _n (rep_type_val g p); gvars gv) 
-        SEP (full_gc g t_info roots outlier ti sh gv)
+        SEP (full_gc g t_info roots outlier ti sh gv * library.mem_mgr gv)
     )
    break: (PROP()LOCAL(temp _i (Vlong (Int64.repr (Z.of_nat n))))
-           SEP(full_gc g t_info roots outlier ti sh gv)).
+           SEP(full_gc g t_info roots outlier ti sh gv * library.mem_mgr gv)).
 - (* Before the loop. *)
   Exists 0%nat. Exists p. rewrite Nat.sub_0_r. entailer!.
   destruct n; constructor.
@@ -103,14 +114,23 @@ Proof.
     entailer!!.
     destruct (n-m)%nat eqn:?H.
     2: contradiction H4; reflexivity.
-    f_equal. f_equal. lia.
+    f_equal. f_equal.
+     lia.
 - (* after the loop *)
- forward.
- apply prop_right.
- f_equal. 
- rewrite Int64.shl_mul_two_p, mul64_repr, add64_repr.
- reflexivity.
-Qed.
+ forward. simpl. 
+Exists (repZ (Z.of_nat n)) g roots t_info.
+ entailer!. split3.
+ + simpl. destruct xs.  unfold FM.from_nat. 
+
+ cbn - [Nat.pow].
+ admit.
+ + apply gc_graph_iso_refl.
+ + simpl. unfold odd_Z2val. simpl.
+ rewrite Int64.shl_mul_two_p, mul64_repr, add64_repr. 
+  unfold two_p. simpl. unfold two_power_pos. simpl.  
+  f_equal. f_equal. lia. 
+ 
+Admitted.
 
 #[export] Instance CCE4: change_composite_env filteredCompSpecs CompSpecs.
 make_cs_preserve filteredCompSpecs CompSpecs.
@@ -147,16 +167,16 @@ Proof.
   - (* During the loop *)
     assert (n - m <> 0)%nat by lia.
     forward_call (gv, g', [v], (m%nat; tt) , roots, sh, ti, outlier, t_info').
-    split; simpl; auto.
+    { split; simpl; auto. }
     Intros v'.  destruct v' as ((v'&g'')&ti').
     unfold fst, snd in *. 
     forward. 
     Exists (v', S m, g'', ti').
     entailer!!.
     split.
-     + eapply gc_graph_iso_trans; eassumption.
-     + repeat f_equal.  lia.
-  -
+     * eapply gc_graph_iso_trans; eassumption.
+     * repeat f_equal.  lia.
+  - (* After the loop *)
     forward.  
     Exists v. Exists g'. Exists t_info'.
     entailer!!.
@@ -169,25 +189,6 @@ Qed.
 #[export] Instance CCE: change_composite_env env_graph_gc.CompSpecs CompSpecs.
 make_cs_preserve env_graph_gc.CompSpecs CompSpecs.
 Defined.
-(*
-#[export] Existing Instance CCE: change_composite_env env_graph_gc.CompSpecs CompSpecs.
-make_cs_preserve env_graph_gc.CompSpecs CompSpecs.
-Defined.
-*)
-
-
-Lemma gc_preserved_nat: 
-  forall outlier (g1 :graph) (roots1: list root_t)
-         (g2: graph) (roots2: list root_t),
-    gc_graph_iso g1 roots1 g2 roots2 ->
-    graph_unmarked g2 /\ no_backward_edge g2 /\ no_dangling_dst g2 ->
-    forall (a: nat) (n: Z),
-      0 <= n < Zlength roots1 ->
-    @graph_predicate _ (@in_graph_pred _ InGraph_nat) g1 outlier a (rep_type_of_root_t (Znth n roots1)) ->
-    @graph_predicate _ (@in_graph_pred _ InGraph_nat) g2 outlier a (rep_type_of_root_t (Znth n roots2)).
-Proof.
-apply @gc_preserved.  (* Kathrin: replace this proof with a real one *)
-Qed.
 
 Lemma test_semax_GC_SAVE1:
  forall (n: Z) (Espec : OracleKind)
@@ -245,16 +246,20 @@ apply_semax_GC_SAVE1.
 simpl app.
 apply andp_left2; repeat (let x := fresh "x" in (Intro x; Exists x));
   go_lowerx; autorewrite with norm; cancel.
-Qed.
+Qed. 
+
 
 Lemma body_uint63_to_nat: semax_body Vprog Gprog f_uint63_to_nat uint63_to_nat_spec.
 Proof. 
-start_function.
+start_function'.
+unfold FM.t in x. destruct x as (n&n_lt).
+cbn in H0. destruct p; try contradiction. subst.
 change (Tpointer _ _) with int_or_ptr_type.
-forward. unfold full_gc. Intros.
+forward.
+unfold full_gc. Intros. 
 forward_call (gv, g, outlier). 
 Intros v.
-rewrite decode_encode_Z by auto.
+(* rewrite decode_encode_Z by auto. *)
 forward.
 forward.
 unfold before_gc_thread_info_rep; limited_change_compspecs CompSpecs.
@@ -267,6 +272,7 @@ sep_apply_compspecs CompSpecs
   (frame_rep__fold Tsh v___FRAME__ v___ROOT__ (ti_fp t_info) 1 (Vlong (Int64.repr 0))).
 sep_apply_compspecs CompSpecs (before_gc_thread_info_rep_fold sh t_info ti).
 sep_apply (full_gc_fold gv g t_info roots outlier ti sh).
+
 forward_while 
 (EX v : rep_type, EX m : nat, EX g' : graph, 
  EX (t_info' : GCGraph.thread_info), EX (roots': roots_t),
@@ -290,57 +296,59 @@ SEP (full_gc g' t_info' roots' outlier ti sh gv;
    split3.
     * apply gc_graph_iso_refl.
     * apply frame_shells_eq_refl.
-    * repeat f_equal. lia.
+    * repeat f_equal. admit. (*  lia. *)
 - (* Valid condition  *)
   entailer!!. 
 - (* During the loop *)
-  rename H4 into GCP. rename H6 into H4.
+  rename H4 into GCP. rename H6 into H_frame_shells.
   assert (STARTptr := space_start_isptr' GCP).
-  assert (m<n)%nat by lia. clear H3 HRE HRE'. rename H6 into HRE.
-  forward.
+  assert (m<n)%nat by lia. clear H3 HRE HRE'. rename H5 into H_iso.
+  forward. 
   eapply semax_seq'.
  + eapply semax_Delta_subsumption with GC_SAVE1_tycontext.
-   apply prove_tycontext_sub; try reflexivity; repeat split; auto.
+   { apply prove_tycontext_sub; try reflexivity; repeat split; auto. }
    apply (@semax_cssub filteredCompSpecs).
-   apply prove_cssub; repeat split; auto; try reflexivity.
+   { apply prove_cssub; repeat split; auto; try reflexivity. }
    change _nalloc with specs_general._nalloc.
    match goal with |- context [full_gc _ _ _ _ ?ti _ _] =>
     match goal with |- context [temp ?tix ti] =>
       change tix with specs_general._tinfo
     end end.
    apply_semax_GC_SAVE1.
-   rewrite Int.signed_repr; rep_lia.
-  + simpl app. 
-   abbreviate_semax.
-  Intros g4 v0' roots4 t_info4.
+   { rewrite Int.signed_repr; rep_lia. }
+  + simpl app. abbreviate_semax.
+  Intros g'' v0' roots'' t_info''.
+  rename H7 into H_iso'. 
   pose (m' := existT (fun _ => unit) m tt).
-  forward_call (gv, g4, [v0'], m', roots4, sh, ti, outlier, t_info4).
-   * split. split; auto. reflexivity. clear - H3.  rewrite Int.signed_repr in H3 by rep_lia. rep_lia.
+  forward_call (gv, g'', [v0'], m', roots'', sh, ti, outlier, t_info'').
+   * split.
+     -- split; auto. reflexivity. 
+     -- clear - H3. rewrite Int.signed_repr in H3 by rep_lia. rep_lia.
    * Intros vret.
-     destruct vret as [[ v2 g5] t_info5].
+     destruct vret as [[ v2 g'''] t_info'''].
      simpl snd in *. simpl fst in *.
-     assert_PROP (gc_condition_prop g5 t_info5 roots4 outlier) as GCP'
+     assert_PROP (gc_condition_prop g''' t_info''' roots'' outlier) as GCP'
         by (unfold full_gc; entailer!!). 
-     simpl in H10.
      forward.
-     Exists (v2, S m,g5,t_info5,roots4). simpl fst. simpl snd.
+     Exists (v2, S m,g''',t_info''',roots''). simpl fst. simpl snd.
+
      unfold ti_fp.
      replace (Z.of_nat (n - S m)) with (Z.of_nat (n-m)-1) by lia.
-     rewrite H13.
+     rewrite H11.
+
      entailer!!.
      split.
-     eapply gc_graph_iso_trans; try eassumption.
-     eapply gc_graph_iso_trans; try eassumption.
-     rewrite <- H13.
-     eapply frame_shells_eq_trans; try eassumption.
+     -- eapply gc_graph_iso_trans; try eassumption.
+     eapply gc_graph_iso_trans; eassumption.
+     -- rewrite <- H11.
+     eapply frame_shells_eq_trans; eassumption.
  - (* after the loop *)
    forward.
    assert (m=n). {
     clear - H3 H HRE. unfold encode_Z in H. 
-    apply repr_inj_unsigned64 in HRE; rep_lia.
-   }
-   subst m.
-   Exists v0 g' t_info' roots'.
+    apply repr_inj_unsigned64 in HRE; try rep_lia. admit.  }
+   subst m. unfold model_fn. simpl.
+   Exists v0 g' roots' t_info' .
    unfold frame_rep_.
-   entailer!!.
-Qed.
+   entailer!!. destruct xs. apply H2. 
+Admitted.
